make frame_typing a Type, fixes in type_progress for lfilled_Ind_Equivalent applications and + vs \/ associativity

theories/pickability.v
@@ -8,8 +8,9 @@ Unset Strict Implicit.
 Unset Printing Implicit Defensive.
 
 (* Basic logic ops for Type *)
-(* TODO move those into a separate file *)
+(* TODO! move those into a separate file *)
 (* XXX is there something similar in stdlib? Search didn't return anything *)
+(* TODO n-ary sigtype notation? *)
 Definition notT (T : Type) : Type := T -> Empty_set.
 Definition decidableT (T : Type) : Type := T + notT T.
 Definition iffT (A B : Type) : Type := prod (A -> B) (B -> A).
@@ -18,6 +19,9 @@ Notation "P <--> Q" := (iffT P Q) (at level 95, right associativity).
  * used this to get not-like behaviour for auto tactics but *)
 Hint Unfold notT : core.
 Hint Unfold iffT : core.
+
+Definition Empty_set_imp_False : Empty_set -> False.
+Proof. intro H. inversion H. Qed.
 
 (** * General lemmas about decidability **)
 
